merge in some changes from main

cedar-lean/Cedar/Partial/Expr.lean
@@ -1,5 +1,5 @@
 /-
- Copyright 2022-2023 Amazon.com, Inc. or its affiliates. All Rights Reserved.
+ Copyright Cedar Contributors
 
  Licensed under the Apache License, Version 2.0 (the "License");
  you may not use this file except in compliance with the License.
@@ -16,11 +16,8 @@
 
 import Cedar.Data
 import Cedar.Spec.Expr
-import Cedar.Thm.Data.Map -- necessary for a termination argument
-import Cedar.Thm.Termination.Expr
-import Cedar.Thm.Termination.Value
 
-/-! This file defines abstract syntax for Cedar expressions. -/
+/-! This file defines abstract syntax for Cedar partial expressions. -/
 
 namespace Cedar.Partial
 
@@ -138,76 +135,46 @@ namespace Cedar.Spec
 
 open Cedar.Data
 
-def Value.asPartialExpr (v : Spec.Value) : Partial.Expr :=
-  match v with
+def Value.asPartialExpr : Spec.Value → Partial.Expr
   | .prim p => .lit p
-  | .set s => .set (s.elts.map₁ λ ⟨v, h₁⟩ =>
-      have := Value.set_termination v s h₁
-      v.asPartialExpr)
-  | .record m => .record (m.kvs.map₁ λ ⟨(k, v), h₁⟩ =>
-      have := Value.record_termination v m (Map.in_kvs_snd_in_values h₁)
-      (k, v.asPartialExpr))
-  | .ext (.decimal d) => .call ExtFun.decimal [Partial.Expr.lit (.string d.unParse)]
-  | .ext (.ipaddr ip) => .call ExtFun.ip [Partial.Expr.lit (.string (Spec.Ext.IPAddr.unParse ip))]
-termination_by v.size
+  | .set (Set.mk elts) => .set (elts.map₁ λ ⟨v, _⟩ => v.asPartialExpr)
+  | .record m => .record (m.kvs.attach₃.map λ ⟨(k, v), _⟩ => (k, v.asPartialExpr))
+  | .ext (.decimal d) => .call ExtFun.decimal [Partial.Expr.lit (.string (toString d))]
+  | .ext (.ipaddr ip) => .call ExtFun.ip [Partial.Expr.lit (.string (toString ip))]
 
-def Value.asPartialRestrictedExpr (v : Spec.Value) : Partial.RestrictedExpr :=
-  match v with
+def Value.asPartialRestrictedExpr : Spec.Value → Partial.RestrictedExpr
   | .prim p => .lit p
-  | .set s => .set (s.elts.map₁ λ ⟨v, h₁⟩ =>
-      have := Value.set_termination v s h₁
+  | .set s => .set (s.elts.map₁ λ ⟨v, _⟩ =>
+      have := Set.sizeOf_lt_of_elts (s := s)
       v.asPartialRestrictedExpr)
-  | .record m => .record (m.kvs.map₁ λ ⟨(k, v), h₁⟩ =>
-      have := Value.record_termination v m (Map.in_kvs_snd_in_values h₁)
-      (k, v.asPartialRestrictedExpr))
-  | .ext (.decimal d) => .call ExtFun.decimal [Value.prim (.string d.unParse)]
-  | .ext (.ipaddr ip) => .call ExtFun.ip [Value.prim (.string (Spec.Ext.IPAddr.unParse ip))]
-termination_by v.size
+  | .record m => .record (m.kvs.attach₂.map λ ⟨(k, v), h₁⟩ => (k, v.asPartialRestrictedExpr))
+  | .ext (.decimal d) => .call ExtFun.decimal [Value.prim (.string (toString d))]
+  | .ext (.ipaddr ip) => .call ExtFun.ip [Value.prim (.string (toString ip))]
+decreasing_by all_goals sorry
 
-def Expr.asPartialExpr (x : Spec.Expr) : Partial.Expr :=
-  match x with
+def Expr.asPartialExpr : Spec.Expr → Partial.Expr
   | .lit p => .lit p
   | .var v => .var v
   | .ite x₁ x₂ x₃ =>
-      have := @Expr.ite_termination x₁ x₂ x₃
       .ite x₁.asPartialExpr x₂.asPartialExpr x₃.asPartialExpr
   | .and x₁ x₂ =>
-      have := @Expr.and_termination x₁ x₂
       .and x₁.asPartialExpr x₂.asPartialExpr
   | .or x₁ x₂ =>
-      have := @Expr.or_termination x₁ x₂
       .or x₁.asPartialExpr x₂.asPartialExpr
   | .unaryApp op x₁ =>
-      have := @Expr.unaryApp_termination x₁ op
       .unaryApp op x₁.asPartialExpr
   | .binaryApp op x₁ x₂ =>
-      have := @Expr.binaryApp_termination x₁ x₂ op
       .binaryApp op x₁.asPartialExpr x₂.asPartialExpr
   | .getAttr x₁ attr =>
-      have := @Expr.getAttr_termination x₁ attr
       .getAttr x₁.asPartialExpr attr
   | .hasAttr x₁ attr =>
-      have := @Expr.hasAttr_termination x₁ attr
       .hasAttr x₁.asPartialExpr attr
   | .set xs =>
-      have h := @Expr.set_termination xs
-      let xs' := xs.map₁ λ ⟨x, prop⟩ =>
-        have := h x prop
-        x.asPartialExpr
-      .set xs'
+      .set (xs.map₁ λ ⟨x, _⟩ => x.asPartialExpr)
   | .record attrs =>
-      have h := @Expr.record_termination attrs
-      let attrs' := attrs.map₁ λ ⟨(k, v), prop⟩ =>
-        have := h (k, v) prop
-        (k, v.asPartialExpr)
-      .record attrs'
+      .record (attrs.attach₂.map λ ⟨(k, v), _⟩ => (k, v.asPartialExpr))
   | .call xfn args =>
-      have h := @Expr.call_termination args xfn
-      let args' := args.map₁ λ ⟨x, prop⟩ =>
-        have := h x prop
-        x.asPartialExpr
-      .call xfn args'
-termination_by x.size
+      .call xfn (args.map₁ λ ⟨x, _⟩ => x.asPartialExpr)
 
 instance : Coe Spec.Expr Partial.Expr where
   coe := Spec.Expr.asPartialExpr
@@ -216,14 +183,12 @@ end Cedar.Spec
 
 namespace Cedar.Partial
 
-def RestrictedExpr.asPartialExpr (x : Partial.RestrictedExpr) : Partial.Expr :=
-  match x with
+def RestrictedExpr.asPartialExpr : Partial.RestrictedExpr → Partial.Expr
   | .lit p => .lit p
-  | .set xs => .set (xs.map Partial.RestrictedExpr.asPartialExpr)
-  | .record attrs => .record (attrs.map λ (k, v) => (k, v.asPartialExpr))
+  | .set xs => .set (xs.map₁ λ ⟨x, _⟩ => x.asPartialExpr)
+  | .record attrs => .record (attrs.attach₂.map λ ⟨(k, v), _⟩ => (k, v.asPartialExpr))
   | .call xfn args => .call xfn (args.map Spec.Value.asPartialExpr)
   | .unknown u => .unknown u
-decreasing_by all_goals sorry
 
 /--
   Is this a literal "unknown".
@@ -250,11 +215,10 @@ def Expr.subexpressions (x : Partial.Expr) : List Partial.Expr :=
   | .binaryApp _ x₁ x₂ => [x] ++ x₁.subexpressions ++ x₂.subexpressions
   | .getAttr x₁ _ => [x] ++ x₁.subexpressions
   | .hasAttr x₁ _ => [x] ++ x₁.subexpressions
-  | .set xs => [x] ++ List.join (xs.map Partial.Expr.subexpressions)
-  | .record pairs => [x] ++ List.join (pairs.map λ (_, x₁) => x₁.subexpressions)
-  | .call _ xs => [x] ++ List.join (xs.map Partial.Expr.subexpressions)
+  | .set xs => [x] ++ List.join (xs.map₁ λ ⟨x, _⟩ => x.subexpressions)
+  | .record pairs => [x] ++ List.join (pairs.attach₂.map λ ⟨(_, x₁), _⟩ => x₁.subexpressions)
+  | .call _ xs => [x] ++ List.join (xs.map₁ λ ⟨x, _⟩ => x.subexpressions)
   | .unknown _ => [x]
-decreasing_by all_goals sorry
 
 /--
   Does a given Partial.Expr contain an Unknown, perhaps recursively
@@ -285,11 +249,10 @@ def RestrictedExpr.isUnknown (x : Partial.RestrictedExpr) : Bool :=
 def RestrictedExpr.subexpressions (x : Partial.RestrictedExpr) : List Partial.RestrictedExpr :=
   match x with
   | .lit _ => [x]
-  | .set xs => [x] ++ List.join (xs.map Partial.RestrictedExpr.subexpressions)
-  | .record pairs => [x] ++ List.join (pairs.map λ (_, x₁) => x₁.subexpressions)
+  | .set xs => [x] ++ List.join (xs.map₁ λ ⟨x, _⟩ => x.subexpressions)
+  | .record pairs => [x] ++ List.join (pairs.attach₂.map λ ⟨(_, x₁), _⟩ => x₁.subexpressions)
   | .call _ xs => [x] -- in Partial.RestrictedExpr, call arguments are values and cannot contain unknowns
   | .unknown _ => [x]
-decreasing_by all_goals sorry
 
 /--
   Does a given Partial.RestrictedExpr contain an Unknown, perhaps recursively
