cedar-lean/Cedar/Thm/Partial/Evaluation/Set.lean
@@ -36,8 +36,9 @@ theorem element_subexpression {x₁ x₂ : Partial.Expr} {xs : List Partial.Expr
   unfold Partial.Expr.subexpressions
   simp [List.append_eq_append]
   right
+  rw [List.map₁_eq_map]
   have h₃ := List.mem_map_of_mem Partial.Expr.subexpressions h₁
-  apply List.mem_join_of_mem h₃ h₂
+  exact List.mem_join_of_mem h₃ h₂
 
 /--
   helper lemma: if any component of a `set` contains an unknown, the whole
